format-version: 1.2
data-version: uberon/releases/2021-07-25/imports/bspo_import.owl
ontology: uberon/imports/bspo_import
property_value: http://purl.org/dc/elements/1.1/source http://purl.obolibrary.org/obo/bspo/releases/2020-05-11/bspo.owl
property_value: owl:versionInfo "2021-07-25" xsd:string

[Term]
id: BSPO:0000054
name: anatomical side
namespace: spatial
def: "An anatomical region bounded by a plane perpendicular to an axis through the middle." [BSPO:cjm]
xref: FBql:00005841
is_a: BSPO:0000070 ! anatomical region

[Term]
id: BSPO:0000059
name: central side
namespace: spatial
def: "Anatomical side that is centrally located on an organism or structure." [BSPO:wd]
comment: central is not an axis direction
synonym: "central" EXACT []
xref: FBcv:0000056
xref: FBql:00015851
is_a: BSPO:0000054 ! anatomical side

[Term]
id: BSPO:0000070
name: anatomical region
namespace: spatial
def: "A 3D region in space without well-defined compartmental boundaries; for example, the dorsal region of an ectoderm." [BSPO:cjm]
comment: to be merged into CARO
xref: FBql:00005841
is_a: CARO:0000003 ! anatomical structure

[Term]
id: BSPO:0000075
name: central region
namespace: spatial
def: "Anatomical region centrally located on the body or body part." [BSPO:wd]
xref: FBql:00015851
is_a: BSPO:0000070 ! anatomical region
intersection_of: BSPO:0000070 ! anatomical region
intersection_of: overlaps BSPO:0000059 ! central side
relationship: overlaps BSPO:0000059 ! central side

[Term]
id: CARO:0000000
name: anatomical entity
namespace: spatial
def: "Biological entity that is either an individual member of a biological species or constitutes the structural organization of an individual member of a biological species." [CARO:MAH]

[Term]
id: CARO:0000003
name: anatomical structure
namespace: spatial
def: "Material anatomical entity that is a single connected structure with inherent 3D shape generated by coordinated expression of the organism's own genome." [CC:DOS]
is_a: CARO:0000006 ! material anatomical entity

[Term]
id: CARO:0000006
name: material anatomical entity
namespace: spatial
def: "An anatomical entity that has mass." [CC:DOS]
is_a: CARO:0000000 ! anatomical entity

[Typedef]
id: aboral_to
name: aboral to
namespace: spatial
def: "nearer to the aboral opening of the organism, on the oral-aboral axis." [BSPO:cjm]
xref: BSPO:0015202
is_transitive: true

[Typedef]
id: adjacent_to
name: adjacent to
namespace: spatial
xref: RO:0002220
is_symmetric: true

[Typedef]
id: anterior_to
name: anterior to
namespace: spatial
def: "x anterior to y iff x is further along the antero-posterior axis than y, towards the head. An antero-posterior axis is an axis that extends through an organism from head end to opposite end of body or tail." [BSPO:cjm]
synonym: "rostral_to" EXACT []
xref: BSPO:0000096
property_value: seeAlso FBcv:0000039
property_value: seeAlso FBql:00005863
is_transitive: true
inverse_of: posterior_to ! posterior to

[Typedef]
id: deep_to
name: deep to
namespace: spatial
def: "Further away from the surface of the organism. Thus, the muscular layer is deep to the skin, but superficial to the intestines." [BSPO:cjm]
xref: BSPO:0000107
is_transitive: true
inverse_of: superficial_to ! superficial to

[Typedef]
id: distal_to
name: distal to
namespace: spatial
def: "x distal to y iff x is further along the proximo-distal axis than y, towards the appendage tip. A proximo-distal axis extends from tip of an appendage (distal) to where it joins the body (proximal)." [BSPO:cjm]
xref: BSPO:0000097
property_value: seeAlso FBcv:0000040
property_value: seeAlso FBql:00005867
is_transitive: true
inverse_of: proximal_to ! proximal to

[Typedef]
id: distalmost_part_of
name: distalmost part of
namespace: spatial
def: "X distalmost part of Y <=> X is in distal side of Y and X is adjacent to the distal boundary of Y" [https://orcid.org/0000-0002-6601-2165]
xref: BSPO:0001108
is_a: in_distal_side_of ! in distal side of

[Typedef]
id: dorsal_to
name: dorsal to
namespace: spatial
def: "x dorsal to y iff x is further along the dorso-ventral axis than y, towards the back. A dorso-ventral axis is an axis that extends through an organism from back (e.g. spinal column) to front (e.g. belly)." [BSPO:cjm]
xref: BSPO:0000098
property_value: seeAlso FBcv:0000041
property_value: seeAlso FBql:00005865
is_transitive: true
inverse_of: ventral_to ! ventral to

[Typedef]
id: has_part
name: has part
namespace: spatial
xref: BFO:0000051
is_transitive: true

[Typedef]
id: immediately_anterior_to
name: immediately anterior to
namespace: spatial
def: "x immediately anterior to y iff x anterior to y and x is contiguous with y." [BSPO:curators]
xref: BSPO:0015009
is_a: anterior_to ! anterior to
inverse_of: immediately_posterior_to ! immediately posterior to

[Typedef]
id: immediately_deep_to
name: immediately deep to
namespace: spatial
def: "x immediately deep to y iff x deep_to y and x is contiguous with y." [BSPO:curators]
xref: BSPO:0001107
is_a: deep_to ! deep to
inverse_of: immediately_superficial_to ! immediately superficial to

[Typedef]
id: immediately_posterior_to
name: immediately posterior to
namespace: spatial
def: "x immediately posterior to y iff x posterior_to y and x is contiguous with y." [BSPO:curators]
xref: BSPO:0015012
is_a: posterior_to ! posterior to

[Typedef]
id: immediately_superficial_to
name: immediately superficial to
namespace: spatial
def: "x immediately superficial to y iff x superficial to y and x is contiguous with y." [BSPO:curators]
xref: BSPO:0015014
is_a: superficial_to ! superficial to

[Typedef]
id: in_anterior_side_of
name: in anterior side of
namespace: spatial
def: "X anterior side of Y <=> if Y is subdivided into two anterior and posterior portions, X is part of the anterior portion." [BSPO:PATO_mtg_2009]
xref: BSPO:0000123
is_a: part_of ! part of

[Typedef]
id: in_deep_part_of
name: in deep part of
namespace: spatial
def: "X superficial part of Y <=> if Y is subdivided into two superficial and deep portions, X is part of the deep portion." [BSPO:cjm]
xref: BSPO:0001101
is_a: part_of ! part of

[Typedef]
id: in_distal_side_of
name: in distal side of
namespace: spatial
def: "x in distal side of y <=> if y is subdivided into two proximal and distal portions, y is part of the distal portion." [BSPO:PATO_mtg_2009]
xref: BSPO:0000125
is_a: part_of ! part of

[Typedef]
id: in_dorsal_side_of
name: in dorsal side of
namespace: spatial
def: "X dorsal side of Y <=> if Y is subdivided into two dorsal and ventral portions, X is part of the dorsal portion." [BSPO:cjm]
xref: BSPO:0015101
is_a: part_of ! part of

[Typedef]
id: in_lateral_side_of
name: in lateral side of
namespace: spatial
def: "X in lateral side of Y <=> if X is in left side of Y or X is in right side of Y. X is often, but not always a paired structure" [UBERON:cjm]
xref: BSPO:0000126
property_value: seeAlso https://github.com/obophenotype/uberon/wiki/Modeling-paired-structures-Design-Pattern xsd:anyURI
is_a: part_of ! part of

[Typedef]
id: in_left_side_of
name: in left side of
namespace: spatial
def: "X in left side of Y <=> if Y is subdivided into two left and right portions, X is part of the left portion." [BSPO:PATO_mtg_2009]
xref: BSPO:0000120
property_value: seeAlso https://github.com/obophenotype/uberon/wiki/Modeling-paired-structures-Design-Pattern xsd:anyURI
is_a: in_lateral_side_of ! in lateral side of
inverse_of: in_right_side_of ! in right side of

[Typedef]
id: in_posterior_side_of
name: in posterior side of
namespace: spatial
def: "X posterior side of Y <=> if Y is subdivided into two anterior and posterior portions, X is part of the posterior portion." [BSPO:PATO_mtg_2009]
xref: BSPO:0000122
is_a: part_of ! part of

[Typedef]
id: in_proximal_side_of
name: in proximal side of
namespace: spatial
def: "x in proximal side of y <=> if y is subdivided into two proximal and distal portions, y is part of the proximal portion." [BSPO:PATO_mtg_2009]
xref: BSPO:0000124
is_a: part_of ! part of

[Typedef]
id: in_right_side_of
name: in right side of
namespace: spatial
def: "X in right side of Y <=> if Y is subdivided into two left and right portions, X is part of the right portion." [BSPO:PATO_mtg_2009]
xref: BSPO:0000121
property_value: seeAlso https://github.com/obophenotype/uberon/wiki/Modeling-paired-structures-Design-Pattern xsd:anyURI
is_a: in_lateral_side_of ! in lateral side of

[Typedef]
id: in_superficial_part_of
name: in superficial part of
namespace: spatial
def: "X superficial part of Y <=> if Y is subdivided into two superficial and deep portions, X is part of the superficial portion." [BSPO:cjm]
xref: BSPO:0001100
is_a: part_of ! part of

[Typedef]
id: in_ventral_side_of
name: in ventral side of
namespace: spatial
def: "X ventral side of Y <=> if Y is subdivided into two dorsal and ventral portions, X is part of the ventral portion." [BSPO:cjm]
xref: BSPO:0015102
is_a: part_of ! part of

[Typedef]
id: intersects_midsagittal_plane_of
name: intersects midsagittal plane of
namespace: spatial
def: "X intersects median plane of iff X crosses the midine plane of Y." []
xref: BSPO:0005001
is_a: part_of ! part of

[Typedef]
id: oral_to
name: oral to
namespace: spatial
def: "nearer to the oral opening of the organism, on the oral-aboral axis." [BSPO:cjm]
xref: BSPO:0015201
is_transitive: true

[Typedef]
id: overlaps
name: overlaps
namespace: spatial
def: "x overlaps y iff they have some part in common." [BSPO:cjm]
comment: "(forall (x y) (iff (overlaps x y) (exists (z) (and (part of z x) (part of z y)))))" CLIF []
xref: RO:0002131

[Typedef]
id: part_of
name: part of
namespace: spatial
xref: BFO:0000050
is_transitive: true
inverse_of: has_part ! has part

[Typedef]
id: postaxial_to
name: postaxial to
namespace: spatial
def: "x preaxial to y iff x is further along the preaxial-postaxial axis than y, towards the postaxial side." [http://medical-dictionary.thefreedictionary.com/postaxial]
synonym: "posterior to (developmentally)" RELATED [MA:th]
xref: BSPO:0001114
is_transitive: true

[Typedef]
id: postaxialmost_part_of
name: postaxialmost part of
namespace: spatial
xref: BSPO:0001115
is_a: part_of ! part of

[Typedef]
id: posterior_to
name: posterior to
namespace: spatial
def: "x posterior to y iff x is further along the antero-posterior axis than y, towards the body/tail. An antero-posterior axis is an axis that extends through an organism from head end to opposite end of body or tail." [BSPO:cjm]
synonym: "caudal to" NARROW vertebrate []
xref: BSPO:0000099
property_value: seeAlso FBcv:0000045
property_value: seeAlso FBql:00005864
is_transitive: true

[Typedef]
id: preaxial_to
name: preaxial to
namespace: spatial
def: "x preaxial to y iff x is further along the preaxial-postaxial axis than y, towards the front." [http://medical-dictionary.thefreedictionary.com/preaxial]
synonym: "anterior to (developmentally)" RELATED [MA:th]
synonym: "lateral (radial) to" RELATED []
synonym: "medial (tibial) to" RELATED []
xref: BSPO:1000000
is_transitive: true

[Typedef]
id: preaxialmost_part_of
name: preaxialmost part of
namespace: spatial
xref: BSPO:0001113
is_a: part_of ! part of

[Typedef]
id: proximal_to
name: proximal to
namespace: spatial
def: "x proximal to y iff x is closer to the point of attachment with the body than y." [BSPO:cjm]
comment: The elbow is proximal to the hand, but distal to the shoulder.
xref: BSPO:0000100
property_value: seeAlso FBcv:0000047
property_value: seeAlso FBql:00005868
is_transitive: true

[Typedef]
id: proximalmost_part_of
name: proximalmost part of
namespace: spatial
def: "X proximalmost part of Y <=> X is in proximal side of Y and X is adjacent to the proximal boundary of Y" [https://orcid.org/0000-0002-6601-2165]
xref: BSPO:0001106
is_a: in_proximal_side_of ! in proximal side of

[Typedef]
id: seeAlso
name: see also
namespace: spatial
xref: http://www.w3.org/2000/01/rdf-schema#seeAlso
is_metadata_tag: true

[Typedef]
id: superficial_to
name: superficial to
namespace: spatial
def: "Near the outer surface of the organism. Thus, skin is superficial to the muscle layer." [BSPO:cjm]
xref: BSPO:0000108
is_transitive: true

[Typedef]
id: ventral_to
name: ventral to
namespace: spatial
def: "x ventral to y iff x is further along the dorso-ventral axis than y, towards the front. A dorso-ventral axis is an axis that extends through an organism from back (e.g. spinal column) to front (e.g. belly)." [BSPO:cjm]
xref: BSPO:0000102
property_value: seeAlso FBcv:0000049
property_value: seeAlso FBql:00005866
is_transitive: true

